examples/NSL/DY.NSL.Protocol.fst
@@ -1,0 +1,167 @@
+module DY.NSL.Protocol
+
+open Comparse
+open DY.Core
+open DY.Lib
+
+open DY.Simplified
+open DY.Extend
+
+open DY.NSL.Data
+
+/// Here, we define the model of the 
+/// Needham-Schroeder-Lowe Fixed Public Key Protocol (NSL)
+///
+/// A -> B: enc{A, N_A}_B       Msg 1
+/// B -> A: enc{B, N_A, N_B}_A  Msg 2
+/// A -> B: enc{N_B}_B          Msg 3
+///
+/// The model consists of 4 functions,
+/// one for each protocol step:
+/// 1. Alice sends the first message to Bob (`send_msg1`)
+/// 2. Bob sends the second message to Alice (`send_msg2`)
+/// 3. Alice sends the third message to Bob (`send_msg3`)
+/// 4. Bob receives the third message from Alice (`receive_msg3`)
+
+(*** Sending the first message (Alice, n_a) ***)
+
+/// Alice sends the first message to Bob:
+/// * Alice generates a new nonce [n_a]
+/// * encrypts the message (Alice, n_a) for Bob
+/// * sends the encrypted message
+/// * stores n_a and Bob in a state (in a new session)
+/// The step returns the ID of the new state
+/// and the timestamp of the message on the trace
+/// The step fails, if
+/// encryption was not successful, i.e.,
+/// Alice does not have a public key of Bob.
+
+val send_msg1: principal -> principal -> state_id -> traceful (option (state_id & timestamp))
+let send_msg1 alice bob alice_public_keys_sid =
+  let* n_a = gen_rand in
+  
+  let msg1 = Msg1 {alice; n_a} in 
+  let*? msg1_encrypted = pke_enc_for alice bob alice_public_keys_sid key_tag msg1 in
+  let* msg_ts = send_msg msg1_encrypted in
+
+  let state = SentMsg1 {bob; n_a} in
+  let* sid = start_new_session alice state in
+
+  return (Some (sid, msg_ts))
+
+(*** Replying to a first message ***)
+
+/// Bob receives the first messages and replies:
+/// * read the message from the trace
+/// * decrypt the message to (Alice, n_a)
+/// * generate a new nonce [n_b]
+/// * encrypt the reply (Bob, n_a, n_b) for Alice
+/// * send the encrypted reply
+/// * store n_a, n_b and Alice in a state in a new session
+/// The step returns the ID of the new state
+/// and the timestamp of the reply on the trace.
+/// The step fails, if one of
+/// * decryption fails
+/// * the message is not of the right type, i.e., not a first message
+/// * encryption fails (for example, if Bob doesn't have a public key for Alice)
+
+val receive_msg1_and_send_msg2: principal -> state_id -> state_id -> timestamp -> traceful (option (state_id & timestamp))
+let receive_msg1_and_send_msg2 bob bob_private_keys_sid bob_public_keys_sid msg_ts =
+  let*? msg = recv_msg msg_ts in
+
+  let*? msg1_ = pke_dec_with_key_lookup #message_t bob bob_private_keys_sid key_tag msg in
+  guard_tr (Msg1? msg1_);*?
+  let Msg1 msg1 = msg1_ in
+  let alice = msg1.alice in
+  let n_a = msg1.n_a in
+
+  let* n_b = gen_rand in
+
+  let msg2 = Msg2 {bob; n_a; n_b} in
+  let*? msg2_encrypted = pke_enc_for bob alice bob_public_keys_sid key_tag msg2 in
+  let* msg2_ts = send_msg msg2_encrypted in
+
+  let state = SentMsg2 {alice; n_a; n_b} in
+  let* sess_id = start_new_session bob state in
+  
+  return (Some (sess_id, msg2_ts))
+
+(*** Sending the final message ***)
+
+
+/// Alice receives the second messages and replies:
+/// * read the message from the trace
+/// * decrypt the message to (Bob, n_a, n_b)
+/// * encrypt the reply (n_b) for Bob
+/// * send the encrypted reply
+/// * store n_a, n_b and Bob in a state in the session related to Bob and n_a
+/// The step returns the ID of the new state
+/// and the timestamp of the reply on the trace.
+/// The step fails, if one of
+/// * decryption fails
+/// * the message is not of the right type, i.e., not a first message
+/// * encryption fails (for example, if Bob doesn't have a public key for Alice)
+/// * there is no prior session related to Bob and n_a
+
+val receive_msg2_and_send_msg3: principal -> state_id -> state_id -> timestamp -> traceful (option (state_id & timestamp))
+let receive_msg2_and_send_msg3 alice alice_private_keys_sid alice_public_keys_sid msg_ts =
+  let*? msg = recv_msg msg_ts in
+
+  let*? msg2_ = pke_dec_with_key_lookup #message_t alice alice_private_keys_sid key_tag msg in
+  guard_tr (Msg2? msg2_);*?
+  let Msg2 msg2 = msg2_ in
+  let bob = msg2.bob in
+  let n_a = msg2.n_a in
+  let n_b = msg2.n_b in
+
+  let*? (sid, st) = lookup_state #state_t alice
+    (fun st -> 
+          SentMsg1? st
+      && (SentMsg1?.sentmsg1 st).n_a = n_a
+      && (SentMsg1?.sentmsg1 st).bob = bob
+    ) in
+  guard_tr(SentMsg1? st);*?
+  
+
+  let msg3 = Msg3 {n_b} in
+  let*? msg3_encrypted = pke_enc_for alice bob alice_public_keys_sid key_tag msg3 in
+  let* msg3_ts = send_msg msg3_encrypted in
+
+  let state = SentMsg3 {bob; n_a; n_b} in
+  set_state alice sid state;*
+  
+  return (Some (sid, msg3_ts))
+
+(*** Receiving the final message ***)
+
+/// Bob receives the reply from Alice:
+/// * read the message from the trace
+/// * decrypt the message to (n_b)
+/// * check if Bob previously sent n_b in some session
+/// * store completion of this session in a new state
+/// Returns the ID of the session that is marked as completed.
+/// The step fails, if one of
+/// * decryption fails
+/// * the message is not of the right type, i.e., not a reply
+/// * there is no prior session related to n_a
+
+val receive_msg3: principal -> state_id -> timestamp -> traceful (option state_id)
+let receive_msg3 bob bob_private_keys_sid msg3_ts =
+  let*? msg = recv_msg msg3_ts in
+  let*? msg3 = pke_dec_with_key_lookup #message_t bob bob_private_keys_sid key_tag msg in
+  guard_tr (Msg3? msg3);*?
+  let Msg3 msg3 = msg3 in
+  let n_b = msg3.n_b in
+
+  let*? (sid, st) = lookup_state #state_t bob
+    (fun st -> 
+          SentMsg2? st
+      && (SentMsg2?.sentmsg2 st).n_b = n_b
+    ) in
+  guard_tr(SentMsg2? st);*?
+  let alice = (SentMsg2?.sentmsg2 st).alice in
+  let n_a = (SentMsg2?.sentmsg2 st).n_a in
+
+  set_state bob sid (ReceivedMsg3 {alice; n_a; n_b});*
+
+  return (Some sid)
