examples/NSL/DY.NSL.Run.Printing.fst
@@ -1,0 +1,38 @@
+module DY.NSL.Run.Printing
+
+open DY.Core
+open DY.Lib
+open Comparse
+
+open DY.Simplified
+
+open DY.NSL.Data
+
+/// Helper functions for trace printing.
+/// Here we define how our abstract message and state types
+/// should be printed.
+
+
+val message_to_string: bytes -> option string
+let message_to_string b =
+  match? parse message_t b with
+  | Msg1 m -> Some (Printf.sprintf "Msg1 [name = (%s), n_a = (%s)]" (m.alice) (bytes_to_string m.n_a))
+  | Msg2 m -> Some (Printf.sprintf "Msg2 [name = (%s), n_a = (%s), n_b = (%s)]" (m.bob) (bytes_to_string m.n_a) (bytes_to_string m.n_b))
+  | Msg3 m -> Some (Printf.sprintf "Msg3 [n_b = (%s)]" (bytes_to_string m.n_b))
+
+
+val state_to_string: bytes -> option string
+let state_to_string b =
+  match? parse state_t b with
+  | SentMsg1 s -> Some (Printf.sprintf "SentMsg1 [n_a = (%s), to = (%s)]" (bytes_to_string s.n_a) s.bob)
+  | SentMsg2 s -> Some (Printf.sprintf "SentMsg2 [n_a = (%s), n_b = (%s), to = (%s)]" (bytes_to_string s.n_a) (bytes_to_string s.n_b) s.alice)
+  | SentMsg3 s -> Some (Printf.sprintf "SentMsg3 [n_a = (%s), n_b = (%s), to = (%s)]" (bytes_to_string s.n_a) (bytes_to_string s.n_b) s.bob)
+  | ReceivedMsg3 s -> Some (Printf.sprintf "ReceivedMsg3 [n_a = (%s), n_b = (%s), from = (%s)]" (bytes_to_string s.n_a) (bytes_to_string s.n_b) s.alice)
+
+
+val get_trace_to_string_printers: trace_to_string_printers
+let get_trace_to_string_printers  = 
+  trace_to_string_printers_builder 
+    message_to_string
+    ((local_state_state_t.tag, state_to_string) :: default_state_to_string)
+    []
