examples/NSL/DY.NSL.Run.fst
@@ -1,0 +1,68 @@
+module DY.NSL.Run
+
+open DY.Core
+open DY.Lib
+
+open DY.Simplified
+
+open DY.NSL.Run.Printing
+open DY.NSL.Data
+open DY.NSL.Protocol
+
+/// Here, we print the trace after a successful run of the NSL protocol.
+
+
+let run () : traceful (option unit ) =
+  let _ = IO.debug_print_string "************* Trace *************\n" in
+
+  (*** Protocol Setup ***)
+
+  // the names of the participants
+  let alice = "Alice" in
+  let bob = "Bob" in
+
+  (*** PKI setup ***)
+
+  // Initialize key storage for Alice
+  // private and public keys are stored in separate sessions
+  let* alice_private_keys_sid = initialize_private_keys alice in
+  let* alice_public_keys_sid = initialize_pki alice in
+
+  // Initialize key storage for Bob
+  let* bob_private_keys_sid = initialize_private_keys bob in
+  let* bob_public_keys_sid = initialize_pki bob in  
+
+  // Generate private key for Alice and store it in her private keys session
+  generate_private_pke_key alice alice_private_keys_sid key_tag;*
+  
+  // Generate private key for Bob and store it in his private keys session
+  generate_private_pke_key bob bob_private_keys_sid key_tag;*
+
+  // Store Bob's public key in Alice's state
+  install_public_pke_key alice alice_public_keys_sid key_tag bob bob_private_keys_sid;*
+
+  // Store Alice's public key in Bob's state
+  install_public_pke_key bob bob_public_keys_sid key_tag alice alice_private_keys_sid;*
+
+  (*** The actual protocol run ***)
+
+  // Alice sends the first message to Bob
+  let*? (alice_sid, msg1_ts) = send_msg1 alice bob alice_public_keys_sid in
+  // Bob replies with a second message (reading Message 1 at the provided timestamp)
+  let*? (bob_sid, msg2_ts) = receive_msg1_and_send_msg2 bob bob_private_keys_sid bob_public_keys_sid msg1_ts in
+  // Alice replies with the third message
+  let*? (alice_sid, msg3_ts) = receive_msg2_and_send_msg3 alice alice_private_keys_sid alice_public_keys_sid msg2_ts in
+  // Bob receives the final message (at the given timestamp)
+  receive_msg3 bob bob_private_keys_sid msg3_ts;*?
+
+
+ (*** Printing the Trace ***)
+
+  let* tr = get_trace in
+  let _ = IO.debug_print_string (
+      trace_to_string get_trace_to_string_printers tr
+    ) in
+
+  return (Some ())
+
+let _ = run () empty_trace
