examples/NSL_with_properties/DY.NSLP.Data.fst
@@ -1,0 +1,186 @@
+module DY.NSLP.Data
+
+open Comparse
+open DY.Core
+open DY.Lib
+
+/// Needham-Schroeder-Lowe Fixed Public Key Protocol [1]
+///
+/// A -> B: {A, N_A}K_PB       Msg 1
+/// B -> A: {B, N_A, N_B}K_PA  Msg 2 -- note addition of B
+/// A -> B: {N_B}K_PB          Msg 3
+///
+/// [1] Gavin Lowe. "Breaking and fixing the Needham-Schroeder Public-Key
+///     Protocol using FDR". TACAS, pp 147-166, 1996.
+///
+/// Here, we define the abstract types for the NSL protocol.
+
+(*** Message Type ***)
+
+/// for each of the messages we define an abstract message type
+
+[@@ with_bytes bytes]
+type message1_t = {
+  alice: principal;
+  n_a: bytes;
+}
+
+[@@ with_bytes bytes]
+type message2_t = {
+  bob: principal;
+  n_a: bytes;
+  n_b: bytes;
+}
+
+[@@ with_bytes bytes]
+type message3_t = {
+  n_b: bytes;
+}
+
+/// the overall abstract message type
+/// (consisting of constructors for the messages
+/// and using the above abstract types for each of them)
+
+[@@ with_bytes bytes]
+type message_t =
+  | Msg1: (m1:message1_t) -> message_t
+  | Msg2: (m2:message2_t) -> message_t
+  | Msg3: (m3:message3_t) -> message_t
+
+/// Using Comparse to generate parser and serializer for the message type
+
+%splice [ps_message1_t] (gen_parser (`message1_t))
+%splice [ps_message2_t] (gen_parser (`message2_t))
+%splice [ps_message3_t] (gen_parser (`message3_t))
+%splice [ps_message_t] (gen_parser (`message_t))
+
+instance parseable_serializeable_bytes_message_t: parseable_serializeable bytes message_t = mk_parseable_serializeable ps_message_t
+
+(*** State Type ***)
+
+/// As for the messages we define abstract state types
+/// for the four states stored by Alice and Bob after each step of the protocol.
+
+[@@ with_bytes bytes]
+type sent_msg1_t  = {
+  bob: principal;
+  n_a: bytes;
+}
+
+[@@ with_bytes bytes]
+type sent_msg2_t  = {
+  alice: principal;
+  n_a: bytes;
+  n_b: bytes;
+}
+
+[@@ with_bytes bytes]
+type sent_msg3_t  = {
+  bob: principal;
+  n_a: bytes;
+  n_b: bytes;
+}
+
+[@@ with_bytes bytes]
+type received_msg3_t  = {
+  alice: principal;
+  n_a: bytes;
+  n_b: bytes;
+}
+
+[@@ with_bytes bytes]
+type state_t =
+  | SentMsg1: (sentmsg1:sent_msg1_t) -> state_t
+  | SentMsg2: (sentmsg2:sent_msg2_t) -> state_t
+  | SentMsg3: (sentmsg3:sent_msg3_t) -> state_t
+  | ReceivedMsg3: (receivedmsg3:received_msg3_t) -> state_t
+
+/// As for messages, we use Comparse to generate
+/// a parser and serializer for our abstract state types.
+
+%splice [ps_sent_msg1_t] (gen_parser (`sent_msg1_t))
+%splice [ps_sent_msg2_t] (gen_parser (`sent_msg2_t))
+%splice [ps_sent_msg3_t] (gen_parser (`sent_msg3_t))
+%splice [ps_received_msg3_t] (gen_parser (`received_msg3_t))
+%splice [ps_state_t] (gen_parser (`state_t))
+
+instance parseable_serializeable_bytes_state_t: parseable_serializeable bytes state_t = mk_parseable_serializeable ps_state_t
+
+
+/// We tag our protocol level states,
+/// so that they are distinguishable from any internal DY* states. 
+
+instance local_state_state_t: local_state state_t = {
+  tag = "NSL.State";
+  format = parseable_serializeable_bytes_state_t;
+}
+
+
+(*** PKI ***)
+
+/// Similarly as for states,
+/// we tag the keys that are used on the protocol level,
+/// so that they can not be confused with other keys.
+
+let key_tag = "NSL.Key"
+
+(*** Event type ***)
+
+/// We have one event per protocol step:
+/// * an Initiating event,
+///   that Alice triggers, when she starts a new run
+/// * a Responding1 event,
+///   that Bob triggers, when he replies to a first message
+/// * a Responding2 event,
+///   that Alice triggers, when she replies to a second message
+/// * a Finishing event,
+///   that Bob triggers, when he receives a final message and finishes the run.
+
+[@@ with_bytes bytes]
+type ev_init_t = {
+  alice:principal;
+  bob:principal;
+  n_a:bytes
+}
+
+[@@ with_bytes bytes]
+type ev_respond1_t = {
+  alice:principal;
+  bob:principal;
+  n_a:bytes;
+  n_b:bytes
+}
+
+[@@ with_bytes bytes]
+type ev_respond2_t = {
+  alice:principal;
+  bob:principal;
+  n_a:bytes;
+  n_b:bytes
+}
+
+[@@ with_bytes bytes]
+type ev_finish_t = {
+  alice:principal;
+  bob:principal;
+  n_a:bytes;
+  n_b:bytes
+}
+
+[@@ with_bytes bytes]
+type event_t =
+  | Initiating:  ev_init_t -> event_t
+  | Responding1: ev_respond1_t -> event_t
+  | Responding2: ev_respond2_t -> event_t
+  | Finishing:   ev_finish_t -> event_t 
+
+%splice [ps_ev_init_t] (gen_parser (`ev_init_t))
+%splice [ps_ev_respond1_t] (gen_parser (`ev_respond1_t))
+%splice [ps_ev_respond2_t] (gen_parser (`ev_respond2_t))
+%splice [ps_ev_finish_t] (gen_parser (`ev_finish_t))
+%splice [ps_event_t] (gen_parser (`event_t))
+
+instance event_event_t: event event_t = {
+  tag = "NSL.Event";
+  format = mk_parseable_serializeable ps_event_t;
+}
