examples/NSL_with_properties/DY.NSLP.Invariants.Proofs.fst
@@ -1,0 +1,307 @@
+module DY.NSLP.Invariants.Proofs
+
+open Comparse
+open DY.Core
+open DY.Lib
+
+open DY.Simplified
+open DY.Extend
+
+open DY.NSLP.Data
+open DY.NSLP.Protocol
+open DY.NSLP.Invariants
+
+#set-options "--fuel 0 --ifuel 1 --z3rlimit 25  --z3cliopt 'smt.qi.eager_threshold=100'"
+
+/// In this module, we show that
+/// the protocol steps maintain the protocol invariants.
+///
+/// For every step s we show a lemma of the form:
+/// trace_invariant tr ==> trace_invariant ( trace after step s )
+
+(*** Sending the First Message ***)
+
+
+val send_msg1_invariant:
+  alice:principal -> bob:principal -> alice_public_keys_sid:state_id ->
+  tr:trace ->
+  Lemma
+  (requires trace_invariant tr)
+  (ensures (
+    let (_ , tr_out) = send_msg1 alice bob alice_public_keys_sid tr in
+    trace_invariant tr_out
+  ))
+let send_msg1_invariant alice bob alice_public_keys_sid tr =
+  let (n_a, tr_rand) = gen_rand_labeled (nonce_label alice bob) tr in
+  let (_, tr_ev) = trigger_event alice (Initiating {alice; bob; n_a}) tr_rand in
+  let msg1 = Msg1 {alice; n_a} in 
+  serialize_wf_lemma message_t (is_knowable_by (nonce_label alice bob) tr_ev) msg1;
+  pke_enc_for_is_publishable tr_ev alice bob alice_public_keys_sid key_tag msg1
+
+(*** Sending the Second Message ***)
+
+
+val decode_msg1_invariant:
+  bob:principal -> bob_private_keys_sid:state_id ->
+  msg:bytes ->
+  tr:trace ->
+  Lemma
+  (requires trace_invariant tr)
+  (ensures (
+    let (_, tr_out) = decode_msg1 bob bob_private_keys_sid msg tr in
+    trace_invariant tr_out
+  ))
+let decode_msg1_invariant bob bob_private_keys_sid msg tr = ()
+
+
+val decode_msg1_proof:
+  bob:principal -> bob_private_keys_sid:state_id ->
+  msg:bytes ->
+  tr:trace ->
+  Lemma
+    (requires 
+       trace_invariant tr /\
+       bytes_invariant tr msg
+    )
+    (ensures (
+      match decode_msg1 bob bob_private_keys_sid msg tr with
+      | (None, _) -> True
+      | (Some {alice; n_a}, _) ->
+          is_knowable_by (nonce_label alice bob) tr n_a
+    ))
+let decode_msg1_proof bob bob_private_keys_sid msg tr =
+      match decode_msg1 bob bob_private_keys_sid msg tr with
+      | (None, _) -> ()
+      | (Some msg1, _) -> (
+          bytes_invariant_pke_dec_with_key_lookup tr #message_t #parseable_serializeable_bytes_message_t bob bob_private_keys_sid key_tag msg;
+          let plain = serialize message_t (Msg1 msg1) in
+          parse_wf_lemma message_t (bytes_invariant tr) plain;
+          FStar.Classical.move_requires (parse_wf_lemma message_t (is_publishable tr)) plain
+      )
+
+val receive_msg1_and_send_msg2_invariant:
+  bob:principal -> 
+  bob_private_keys_sid:state_id -> bob_public_keys_sid:state_id ->
+  msg_ts:timestamp -> 
+  tr:trace ->
+  Lemma
+  (requires trace_invariant tr)
+  (ensures (
+    let (_ , tr_out) = receive_msg1_and_send_msg2 bob bob_private_keys_sid bob_public_keys_sid msg_ts tr in
+    trace_invariant tr_out
+  ))
+let receive_msg1_and_send_msg2_invariant bob bob_private_keys_sid bob_public_keys_sid msg_ts tr =
+  match recv_msg msg_ts tr with
+  | (None, _ ) -> ()
+  | (Some msg, _) -> (
+      match decode_msg1 bob bob_private_keys_sid msg tr with
+      | (None, _) -> ()
+      | (Some msg1, _) -> (
+          let alice = msg1.alice in
+          let n_a = msg1.n_a in
+          
+          let (n_b, tr_rand) = gen_rand_labeled (nonce_label alice bob) tr in
+          assert(trace_invariant tr_rand);
+          
+          let (_, tr_ev) = trigger_event bob (Responding1 {alice; bob; n_a; n_b}) tr_rand in
+          assert(trace_invariant tr_ev);
+          
+          let msg2 = Msg2 {bob; n_a; n_b} in
+          match pke_enc_for bob alice bob_public_keys_sid key_tag msg2 tr_ev with
+          | (None, _) -> ()
+          | (Some msg2_encrypted, tr_msg2) ->(
+              assert(trace_invariant tr_msg2);
+              
+              let (msg2_ts, tr_msg2_) = send_msg msg2_encrypted tr_msg2 in
+                decode_msg1_proof bob bob_private_keys_sid msg tr;
+                serialize_wf_lemma message_t (is_knowable_by (nonce_label alice bob) tr_rand) msg2;
+                pke_enc_for_is_publishable tr_ev bob alice bob_public_keys_sid key_tag msg2;
+              assert(trace_invariant tr_msg2_);
+              
+              let state = SentMsg2 {alice; n_a; n_b} in
+              let (sess_id, tr_sess) = start_new_session bob state tr_msg2_ in
+              assert(trace_invariant tr_sess)
+          )
+      )
+  )
+
+(*** Sending the Third Message ***)
+
+val decode_msg2_invariant:
+  alice:principal -> alice_private_keys_sid:state_id ->
+  msg:bytes ->
+  tr:trace ->
+  Lemma
+  (requires trace_invariant tr)
+  (ensures (
+    let (_, tr_out) = decode_msg2 alice alice_private_keys_sid msg tr in
+    trace_invariant tr_out
+  ))
+let decode_msg2_invariant alice alice_private_keys_sid msg tr = ()
+
+val decode_msg2_proof:
+  alice:principal -> alice_private_keys_sid:state_id ->
+  msg:bytes ->
+  tr:trace ->
+  Lemma
+  (requires 
+     trace_invariant tr /\
+     bytes_invariant tr msg
+  )
+  (ensures (
+    match decode_msg2 alice alice_private_keys_sid msg tr with
+    | (None, _) -> True
+    | (Some {bob; n_a; n_b}, _) -> (
+        is_knowable_by (nonce_label alice bob) tr n_b /\
+        ( is_publishable tr n_a \/
+          event_triggered tr bob (Responding1 {alice; bob; n_a; n_b}))
+     )
+  ))
+let decode_msg2_proof alice alice_private_keys_sid msg tr =
+  match decode_msg2 alice alice_private_keys_sid msg tr with
+  | (None, _) -> ()
+  | (Some msg2, _) -> (
+      bytes_invariant_pke_dec_with_key_lookup tr #message_t #parseable_serializeable_bytes_message_t alice alice_private_keys_sid key_tag msg;
+      let plain = serialize message_t (Msg2 msg2) in
+      parse_wf_lemma message_t (bytes_invariant tr) plain;
+      FStar.Classical.move_requires (parse_wf_lemma message_t (is_publishable tr)) plain
+  )  
+
+#push-options "--z3rlimit 50"
+val receive_msg2_and_send_msg3_invariant:
+  alice:principal -> 
+  alice_private_keys_sid:state_id -> alice_public_keys_sid:state_id ->
+  msg_ts:timestamp -> 
+  tr:trace ->
+  Lemma
+  (requires trace_invariant tr)
+  (ensures (
+    let (_ , tr_out) = receive_msg2_and_send_msg3 alice alice_private_keys_sid alice_public_keys_sid msg_ts tr in
+    trace_invariant tr_out
+  ))
+let receive_msg2_and_send_msg3_invariant alice alice_private_keys_sid alice_public_keys_sid msg_ts tr =
+  match recv_msg msg_ts tr with
+  | (None, _) -> ()
+  | (Some msg2_, _) -> (
+      match decode_msg2 alice alice_private_keys_sid msg2_ tr with
+      | (None, _ ) -> ()
+      | (Some msg2, _) -> (
+            let bob = msg2.bob in
+            let n_a = msg2.n_a in
+            let n_b = msg2.n_b in
+
+            let p = (fun (st:state_t) -> 
+                        SentMsg1? st
+                    && (SentMsg1?.sentmsg1 st).n_a = n_a
+                    && (SentMsg1?.sentmsg1 st).bob = bob
+                    ) in
+            match lookup_state #state_t alice p tr with
+            | (None, _) -> ()
+            | (Some (sid, st), _ ) -> (
+                 let ((), tr_ev) = trigger_event alice (Responding2 {alice; bob; n_a; n_b}) tr in
+                   decode_msg2_proof alice alice_private_keys_sid msg2_ tr;
+                 assert(trace_invariant tr_ev);
+                 
+                 let msg3 = Msg3 {n_b} in
+                 match pke_enc_for alice bob alice_public_keys_sid key_tag msg3 tr_ev with
+                 | (None, _ ) -> ()
+                 | (Some msg3_encrypted, tr_enc) -> (
+                      assert(trace_invariant tr_enc);
+                      
+                      let (_, tr_msg3) = send_msg msg3_encrypted tr_enc in
+                        serialize_wf_lemma message_t (is_knowable_by (nonce_label alice bob) tr) msg3;
+                        pke_enc_for_is_publishable tr_ev alice bob alice_public_keys_sid key_tag msg3; 
+                      assert(trace_invariant tr_msg3);
+                      
+                      let state = SentMsg3 {bob; n_a; n_b} in
+                      let ((), tr_st) = set_state alice sid state tr_msg3 in
+                      assert(trace_invariant tr_st)
+                 )
+            )
+      )
+  )
+#pop-options
+
+(*** Receiving the Final Message ***)
+
+
+val decode_msg3_invariant:
+  bob:principal -> bob_private_keys_sid:state_id ->
+  msg:bytes ->
+  tr:trace ->
+  Lemma
+  (requires trace_invariant tr)
+  (ensures (
+    let (_, tr_out) = decode_msg3 bob bob_private_keys_sid msg tr in
+    trace_invariant tr_out
+  ))
+let decode_msg3_invariant bob bob_private_keys_sid msg tr = ()
+
+val decode_msg3_proof:
+  bob:principal -> bob_private_keys_sid:state_id ->
+  msg:bytes ->
+  tr:trace ->
+  Lemma
+  (requires 
+     trace_invariant tr /\
+     bytes_invariant tr msg
+  )
+  (ensures (
+    match decode_msg3 bob bob_private_keys_sid msg tr with
+    | (None, _) -> True
+    | (Some {n_b}, _) -> (
+         is_publishable tr n_b \/ (
+            exists alice n_a.
+                get_label tr n_b `can_flow tr` (nonce_label alice bob) /\
+                event_triggered tr alice (Responding2 {alice; bob; n_a; n_b})
+         )
+      )
+  ))
+let decode_msg3_proof bob bob_private_keys_sid msg tr = 
+  match decode_msg3 bob bob_private_keys_sid msg tr with
+  | (None, _) -> ()
+  | (Some msg3, _) -> (
+      bytes_invariant_pke_dec_with_key_lookup tr #message_t #parseable_serializeable_bytes_message_t bob bob_private_keys_sid key_tag msg;
+      let plain = serialize message_t (Msg3 msg3) in
+      parse_wf_lemma message_t (bytes_invariant tr) plain;
+      FStar.Classical.move_requires (parse_wf_lemma message_t (is_publishable tr)) plain
+  )  
+
+val receive_msg3_invariant:
+  bob:principal ->
+  bob_private_keys_sid:state_id ->
+  msg_ts:timestamp ->
+  tr:trace ->
+  Lemma
+  (requires trace_invariant tr)
+  (ensures (
+    let (_, tr_out) = receive_msg3 bob bob_private_keys_sid msg_ts tr in
+    trace_invariant tr_out
+  ))
+let receive_msg3_invariant bob bob_private_keys_sid msg_ts tr = 
+  match recv_msg msg_ts tr with
+  | (None, _ ) -> ()
+  | (Some msg3_, _) -> (
+       match decode_msg3 bob bob_private_keys_sid msg3_ tr with
+       | (None, _ ) -> ()
+       | (Some msg3, _) -> (
+            let n_b = msg3.n_b in
+            let p = (fun (st:state_t) -> 
+                        SentMsg2? st
+                    && (SentMsg2?.sentmsg2 st).n_b = n_b
+                    ) in
+            match lookup_state #state_t bob p tr with
+            | (None, _ ) -> ()
+            | (Some (sid, st), _ ) -> (
+                 let alice = (SentMsg2?.sentmsg2 st).alice in
+                 let n_a = (SentMsg2?.sentmsg2 st).n_a in
+
+                 let (_, tr_ev) = trigger_event bob (Finishing {alice; bob; n_a; n_b}) tr in
+                   decode_msg3_proof bob bob_private_keys_sid msg3_ tr;
+                 assert(trace_invariant tr_ev);
+                 
+                 let (_, tr_st) = set_state bob sid (ReceivedMsg3 {alice; n_a; n_b}) tr_ev in
+                 assert(trace_invariant tr_st)
+            )
+       )
+  )
