examples/NSL_with_properties/DY.NSLP.Invariants.fst
@@ -1,0 +1,198 @@
+module DY.NSLP.Invariants
+
+open Comparse
+open DY.Core
+open DY.Lib
+open DY.Extend
+
+open DY.NSLP.Data
+open DY.NSLP.Protocol
+
+#set-options "--fuel 0 --ifuel 1 --z3rlimit 25  --z3cliopt 'smt.qi.eager_threshold=100'"
+
+/// This module defines the protocol invariants,
+/// consisting of:
+/// * the crypto invariants
+/// * trace invariants:
+///   * state invariants
+///   * event invariants
+
+(*** Crypto Invariants ***)
+
+%splice [ps_message1_t_is_well_formed] (gen_is_well_formed_lemma (`message1_t))
+%splice [ps_message2_t_is_well_formed] (gen_is_well_formed_lemma (`message2_t))
+%splice [ps_message3_t_is_well_formed] (gen_is_well_formed_lemma (`message3_t))
+%splice [ps_message_t_is_well_formed] (gen_is_well_formed_lemma (`message_t))
+
+instance crypto_usages_nsl : crypto_usages = default_crypto_usages
+
+#push-options "--ifuel 3"
+val crypto_predicates_nsl: crypto_predicates
+let crypto_predicates_nsl = {
+  default_crypto_predicates with
+  pke_pred = {
+    pred = (fun tr sk_usage pk msg ->
+      (exists prin. 
+        sk_usage == long_term_key_type_to_usage (LongTermPkeKey key_tag) prin /\ 
+      (match parse message_t msg with
+        | Some (Msg1 {alice; n_a}) -> (
+          let bob = prin in
+          get_label tr n_a == nonce_label alice bob /\
+          event_triggered tr alice (Initiating {alice; bob; n_a})
+        )
+        | Some (Msg2 {bob; n_a; n_b}) -> (
+          let alice = prin in
+          get_label tr n_b == nonce_label alice bob /\
+          event_triggered tr bob (Responding1 {alice; bob; n_a; n_b})
+        )
+        | Some (Msg3 {n_b}) -> (
+          let bob = prin in
+          exists alice n_a.
+            get_label tr n_b `can_flow tr` (nonce_label alice bob) /\
+            event_triggered tr alice (Responding2 {alice; bob; n_a; n_b})
+        )
+        | None -> False
+      ))
+    );
+    pred_later = (fun tr1 tr2 sk_usage pk msg ->
+      parse_wf_lemma message_t (bytes_well_formed tr1) msg
+    );
+  };
+}
+#pop-options
+
+instance crypto_invariants_nsl: crypto_invariants = {
+  usages = crypto_usages_nsl;
+  preds =  crypto_predicates_nsl
+}
+
+
+(*** State Invariant ***)
+
+%splice [ps_sent_msg1_t_is_well_formed] (gen_is_well_formed_lemma (`sent_msg1_t))
+%splice [ps_sent_msg2_t_is_well_formed] (gen_is_well_formed_lemma (`sent_msg2_t))
+%splice [ps_sent_msg3_t_is_well_formed] (gen_is_well_formed_lemma (`sent_msg3_t))
+%splice [ps_received_msg3_t_is_well_formed] (gen_is_well_formed_lemma (`received_msg3_t))
+%splice [ps_state_t_is_well_formed] (gen_is_well_formed_lemma (`state_t))
+
+/// The (local) state predicate.
+
+#push-options "--ifuel 2"
+let state_predicate_nsl: local_state_predicate state_t = {
+  pred = (fun tr prin sess_id st ->
+    match st with
+    | SentMsg1 {bob; n_a} -> (
+      let alice = prin in
+      is_knowable_by (nonce_label alice bob) tr n_a /\
+      event_triggered tr alice (Initiating {alice; bob; n_a})
+    )
+    | SentMsg2 {alice; n_a; n_b} -> (
+      let bob = prin in
+      is_knowable_by (nonce_label alice bob) tr n_a /\
+      is_knowable_by (nonce_label alice bob) tr n_b /\
+      event_triggered tr bob (Responding1 {alice; bob; n_a; n_b})
+    )
+    | SentMsg3 {bob; n_a; n_b}  -> (
+      let alice = prin in
+      is_knowable_by (nonce_label alice bob) tr n_a /\
+      is_knowable_by (nonce_label alice bob) tr n_b /\
+      event_triggered tr alice (Responding2 {alice; bob; n_a; n_b})
+    )
+    | ReceivedMsg3 {alice; n_a; n_b} -> (
+      let bob = prin in
+      is_knowable_by (nonce_label alice bob) tr n_a /\
+      is_knowable_by (nonce_label alice bob) tr n_b /\
+      event_triggered tr bob (Finishing {alice; bob; n_a; n_b} )
+    )
+  );
+  pred_later = (fun tr1 tr2 prin sess_id st -> ());
+  pred_knowable = (fun tr prin sess_id st -> ());
+}
+#pop-options
+
+(*** Event Predicate ***)
+
+
+let event_predicate_nsl: event_predicate event_t =
+  fun tr prin e ->
+    match e with
+    | Initiating {alice; bob; n_a} -> (
+      prin == alice /\
+      is_secret (nonce_label alice bob) tr n_a /\
+      rand_just_generated tr n_a
+    )
+    | Responding1 {alice; bob; n_a; n_b} -> (
+      prin == bob /\
+      is_secret (nonce_label alice bob) tr n_b /\
+      rand_just_generated tr n_b
+    )
+    | Responding2 {alice; bob; n_a; n_b} -> (
+      prin == alice /\
+      event_triggered tr alice (Initiating {alice; bob; n_a}) /\ (
+        is_publishable tr n_a \/
+        event_triggered tr bob (Responding1 {alice; bob; n_a; n_b})
+      )
+    )
+    | Finishing {alice; bob; n_a; n_b} -> (
+      prin == bob /\
+      event_triggered tr bob (Responding1 {alice; bob; n_a; n_b}) /\ (
+        is_publishable tr n_b \/
+        event_triggered tr alice (Responding2 {alice; bob; n_a; n_b})
+      )
+    )
+
+/// List of all local state predicates.
+
+let all_sessions = [
+  pki_tag_and_invariant;
+  private_keys_tag_and_invariant;
+  (|local_state_state_t.tag, local_state_predicate_to_local_bytes_state_predicate state_predicate_nsl|);
+]
+
+/// List of all local event predicates.
+
+let all_events = [
+  (event_event_t.tag, compile_event_pred event_predicate_nsl)
+]
+
+/// Create the global trace invariants.
+
+let trace_invariants_nsl: trace_invariants = {
+  state_pred = mk_state_pred all_sessions;
+  event_pred = mk_event_pred all_events;
+}
+
+instance protocol_invariants_nsl: protocol_invariants = {
+  crypto_invs = crypto_invariants_nsl;
+  trace_invs = trace_invariants_nsl;
+}
+
+/// Lemmas that the global state predicate contains all the local ones
+
+val all_sessions_has_all_sessions: unit -> Lemma (norm [delta_only [`%all_sessions; `%for_allP]; iota; zeta] (for_allP (has_local_bytes_state_predicate #protocol_invariants_nsl) all_sessions))
+let all_sessions_has_all_sessions () =
+  assert_norm(List.Tot.no_repeats_p (List.Tot.map dfst (all_sessions)));
+  mk_state_pred_correct #protocol_invariants_nsl all_sessions;
+  norm_spec [delta_only [`%all_sessions; `%for_allP]; iota; zeta] (for_allP (has_local_bytes_state_predicate #protocol_invariants_nsl) all_sessions)
+
+val protocol_invariants_nsl_has_pki_invariant: squash (has_pki_invariant #protocol_invariants_nsl)
+let protocol_invariants_nsl_has_pki_invariant = all_sessions_has_all_sessions ()
+
+val protocol_invariants_nsl_has_private_keys_invariant: squash (has_private_keys_invariant #protocol_invariants_nsl)
+let protocol_invariants_nsl_has_private_keys_invariant = all_sessions_has_all_sessions ()
+
+val protocol_invariants_nsl_has_nsl_session_invariant: squash (has_local_state_predicate state_predicate_nsl)
+let protocol_invariants_nsl_has_nsl_session_invariant = all_sessions_has_all_sessions ()
+
+/// Lemmas that the global event predicate contains all the local ones
+
+val all_events_has_all_events: unit -> Lemma (norm [delta_only [`%all_events; `%for_allP]; iota; zeta] (for_allP (has_compiled_event_pred #protocol_invariants_nsl) all_events))
+let all_events_has_all_events () =
+  assert_norm(List.Tot.no_repeats_p (List.Tot.map fst (all_events)));
+  mk_event_pred_correct #protocol_invariants_nsl all_events;
+  norm_spec [delta_only [`%all_events; `%for_allP]; iota; zeta] (for_allP (has_compiled_event_pred #protocol_invariants_nsl) all_events);
+  let dumb_lemma (x:prop) (y:prop): Lemma (requires x /\ x == y) (ensures y) = () in
+  dumb_lemma (for_allP (has_compiled_event_pred #protocol_invariants_nsl) all_events) (norm [delta_only [`%all_events; `%for_allP]; iota; zeta] (for_allP (has_compiled_event_pred #protocol_invariants_nsl) all_events))
+
+val protocol_invariants_nsl_has_nsl_event_invariant: squash (has_event_pred event_predicate_nsl)
+let protocol_invariants_nsl_has_nsl_event_invariant = all_events_has_all_events ()
