examples/NSL_with_properties/DY.NSLP.Properties.fst
@@ -1,0 +1,94 @@
+module DY.NSLP.Properties
+
+open Comparse
+open DY.Core
+open DY.Lib
+open DY.Extend
+open DY.Simplified
+
+open DY.NSLP.Data
+open DY.NSLP.Invariants
+
+#set-options "--fuel 0 --ifuel 1 --z3rlimit 25  --z3cliopt 'smt.qi.eager_threshold=100'"
+
+/// This module defines the security properties of the NSL protocol:
+/// * secrecy of both nonces
+/// * authentication of both participants
+
+
+/// The nonce n_a is unknown to the attacker,
+/// unless the attacker corrupted Alice or Bob.
+
+val n_a_secrecy:
+  tr:trace -> alice:principal -> bob:principal -> n_a:bytes ->
+  Lemma
+  (requires
+    trace_invariant tr /\ (
+      (state_was_set_some_id tr alice (SentMsg1 {bob; n_a})) \/
+      (exists n_b. state_was_set_some_id tr alice (SentMsg3 {bob; n_a; n_b})) \/
+      (exists n_b. state_was_set_some_id tr bob (ReceivedMsg3 {alice; n_a; n_b}))
+    ) /\
+    attacker_knows tr n_a
+  )
+  (ensures principal_is_corrupt tr alice \/ principal_is_corrupt tr bob)
+let n_a_secrecy tr alice bob n_a =
+  attacker_only_knows_publishable_values tr n_a
+
+/// The nonce n_b is unknown to the attacker,
+/// unless the attacker corrupted Alice or Bob.
+
+val n_b_secrecy:
+  tr:trace -> alice:principal -> bob:principal -> n_b:bytes ->
+  Lemma
+  (requires
+    attacker_knows tr n_b /\
+    trace_invariant tr /\ (
+      (exists n_a. state_was_set_some_id tr bob (SentMsg2 {alice; n_a; n_b})) \/
+      (exists n_a. state_was_set_some_id tr bob (ReceivedMsg3 {alice; n_a; n_b})) \/
+      (exists n_a. state_was_set_some_id tr alice (SentMsg3 {bob; n_a; n_b}))
+    )
+  )
+  (ensures principal_is_corrupt tr alice \/ principal_is_corrupt tr bob)
+let n_b_secrecy tr alice bob n_b =
+  attacker_only_knows_publishable_values tr n_b
+
+
+/// If Bob thinks he talks with Alice,
+/// then Alice thinks she talks to Bob (with the same nonces),
+/// unless the attacker corrupted Alice or Bob.
+
+val initiator_authentication:
+  tr:trace -> ts:timestamp ->
+  alice:principal -> bob:principal -> n_a:bytes -> n_b:bytes ->
+  Lemma
+  (requires
+    event_triggered_at tr ts bob (Finishing {alice; bob; n_a; n_b}) /\
+    trace_invariant tr
+  )
+  (ensures
+    principal_is_corrupt tr alice \/
+    principal_is_corrupt tr bob \/ (
+      event_triggered_before tr ts alice (Responding2 {alice; bob; n_a; n_b}) /\
+      event_triggered_before tr ts alice (Initiating {alice; bob; n_a})
+    )
+  )
+let initiator_authentication tr ts alice bob n_a n_b = ()
+
+/// If Alice thinks she talks with Bob,
+/// then Bob thinks he talks to Alice (with the same nonces),
+/// unless the attacker corrupted Alice or Bob.
+
+val responder_authentication:
+  tr:trace -> ts:timestamp ->
+  alice:principal -> bob:principal -> n_a:bytes -> n_b:bytes ->
+  Lemma
+  (requires
+    event_triggered_at tr ts alice (Responding2 {alice; bob; n_a; n_b}) /\
+    trace_invariant tr
+  )
+  (ensures
+    principal_is_corrupt tr alice \/
+    principal_is_corrupt tr bob \/
+    event_triggered_before tr ts bob (Responding1 {alice; bob; n_a; n_b})
+  )
+let responder_authentication tr ts alice bob n_a n_b = ()
